examples/zip_reverse_r.v
@@ -1,0 +1,63 @@
+From Stdlib Require Import List String ZArith.
+From shift_reset.core Require Import syntax syntax_notation coerce.
+From shift_reset.interpreter Require Import interpreter error.
+From examples.lib Require Import list.
+Import ListNotations.
+
+Open Scope Z_scope.
+Open Scope string_scope.
+Open Scope term_scope.
+
+Example zip_reverse_r :=
+  <{ fun "args" =>
+       let ("xs", "ys") := "args" in
+       let fix "go" "xs" :=
+         match "xs" with
+         | Inl _ => ("ys", Inl ())
+         | Inr "p" =>
+             let ("x", "xs'") := "p" in
+             let "p" := "go" "xs'" in
+             let ("ys_r", "r") := "p" in
+             match "ys_r" with
+             | Inl _ => "p"
+             | Inr "p" =>
+                 let ("y", "ys_r'") := "p" in
+                 ("ys_r'", Inr (("x", "y"), "r"))
+             end
+         end
+       in
+       let "p" := "go" "xs" in
+       snd "p" }>.
+
+Example zip_reverse_r' :=
+  <{ fun "args" =>
+       let ("xs", "ys") := "args" in
+       let fix "go" "args" :=
+         let ("ys", "k") := "args" in
+         match "ys" with
+         | Inl _ => "k"
+         | Inr "p" =>
+             let ("y", "ys'") := "p" in
+             "go" ("ys'", fun "xs" =>
+                            match "xs" with
+                            | Inl _ => Inl ()
+                            | Inr "p" =>
+                                let ("x", "xs'") := "p" in
+                                let "r" := "k" "xs'" in
+                                Inr (("x", "y"), "r")
+                            end)
+         end
+       in
+       let "k" := "go" ("ys", fun _ => Inl ()) in
+       "k" "xs" }>.
+
+Definition eval_zip_reverse_r (candidate : val_term) (fuel : nat) (xs ys : list Z) :=
+  eval_term_to_list
+    (fun v => match v with
+              | VPair (VInt z1) (VInt z2) => inr (z1, z2)
+              | _ => inl (Reflect_failure v)
+              end)
+    fuel <{ candidate ({list_int_to_val_term xs}, {list_int_to_val_term ys}) }>.
+
+Compute (eval_zip_reverse_r zip_reverse_r 100 [1; 2] [3; 4]).
+Compute (eval_zip_reverse_r zip_reverse_r' 100 [1; 2] [3; 4]).
