shift-reset/lib/sum.v
@@ -1,10 +1,10 @@
+Definition pure {A B} : B -> A + B := inr.
+
 Definition map {A B C} (f : B -> C) (s : A + B) : A + C :=
   match s with
   | inl e => inl e
   | inr x => inr (f x)
   end.
-
-Definition pure {A B} : B -> A + B := inr.
 
 Definition bind {A B C} (s : A + B) (f : B -> A + C) : A + C :=
   match s with
@@ -25,3 +25,15 @@ Lemma eq_dec :
          (s1 s2 : A + B),
     {s1 = s2} + {s1 <> s2}.
 Proof. decide equality. Defined.
+
+Module SumNotations.
+  Declare Scope sum_scope.
+  Delimit Scope sum_scope with sum.
+  Bind Scope sum_scope with sum.
+
+  Notation "f <$> m" := (map f m) (at level 65, right associativity) : sum_scope.
+  Notation "m >>= f" := (bind m f) (at level 50, left associativity) : sum_scope.
+
+  Notation "let+ x := m 'in' k" := (map (fun x => k) m) (at level 100, x binder, right associativity) : sum_scope.
+  Notation "let* x := m 'in' k" := (bind m (fun x => k)) (at level 100, x binder, right associativity) : sum_scope.
+End SumNotations.
